theories/FormalSQL/RewriteSpec.v
@@ -12,42 +12,42 @@ Import Tuple.
   workspace, not as axioms in this library.
 *)
 
-Definition select_list_directly_preserves_attr
+Definition select_list_directly_selects_attr
     (s : SelectListT) (a : attribute TNull) : Prop :=
   match s with
   | @_Select_List _ l => In (@Select_As TNull (@A_Expr TNull (@F_Dot TNull a)) a) l
   end.
 
-Definition select_list_outputs_distinct_attrs (s : SelectListT) : Prop :=
+Definition select_list_has_unique_outputs (s : SelectListT) : Prop :=
   match s with
   | @_Select_List _ l => all_diff (map fst (map (@pair_of_select TNull) l))
   end.
 
-Definition projection_preserves_attr_value
+Definition projection_preserves_attr
     (env : Env.env TNull) (s : SelectListT) (a : attribute TNull) : Prop :=
   forall t, a inS labels TNull t -> @dot TNull (projected_tuple env s t) a = @dot TNull t a.
 
-Definition select_list_preserves_formula
+Definition select_list_preserves_formula_eval
     (db : db_state) (s : SelectListT) (f : Formula) : Prop :=
   forall t,
     eval_formula_in_state db (projected_tuple nil s t) f =
     eval_formula_in_state db t f.
 
-Definition formula_implies_on_output
+Definition query_entails
     (db : db_state) (q : Query) (premise conclusion : Formula) : Prop :=
   forall t,
     t inBE eval_query_in_state db q ->
     eval_formula_in_state db t premise = true ->
     eval_formula_in_state db t conclusion = true.
 
-Lemma direct_projection_preserves_attr_value :
+Lemma direct_projection_preserves_attr :
   forall env s a,
-    select_list_directly_preserves_attr s a ->
-    select_list_outputs_distinct_attrs s ->
-    projection_preserves_attr_value env s a.
+    select_list_directly_selects_attr s a ->
+    select_list_has_unique_outputs s ->
+    projection_preserves_attr env s a.
 Proof.
 intros env [l] a Hpres Hdistinct t Ha.
-unfold projection_preserves_attr_value, projected_tuple in *.
+unfold projection_preserves_attr, projected_tuple in *.
 change (@dot TNull (projection TNull (env_t TNull env t) (@Select_List TNull (@_Select_List TNull l))) a = @dot TNull t a).
 rewrite (@dot_projection TNull (env_t TNull env t) l a (@A_Expr TNull (@F_Dot TNull a)) Hpres Hdistinct).
 unfold Interp.interp_aggterm, Interp.interp_funterm, Interp.interp_dot, env_t.
@@ -59,7 +59,7 @@ rewrite Ha.
 apply refl_equal.
 Qed.
 
-Lemma eval_formula_in_env_eq :
+Lemma eval_formula_in_env_eq_tuple :
   forall db env f t1 t2,
     t1 =t= t2 ->
     eval_formula_in_env db env t1 f = eval_formula_in_env db env t2 f.
@@ -76,12 +76,12 @@ apply (@is_true_eval_f_eq
   env f t1 t2 Ht).
 Qed.
 
-Lemma selected_rows_satisfy_filter :
+Lemma sigma_outputs_satisfy_predicate :
   forall db q f,
-    formula_true_on_output db (Sigma f q) f.
+    query_satisfies db (Sigma f q) f.
 Proof.
 intros db q f t Ht.
-unfold formula_true_on_output in *.
+unfold query_satisfies in *.
 unfold eval_query_in_state, eval_formula_in_state, Sigma in Ht |- *.
 unfold eval_query_in_env in Ht.
 rewrite eval_query_unfold in Ht.
@@ -103,10 +103,10 @@ rewrite Febag.mem_filter in Ht.
     nil f t1 t2 Ht12).
 Qed.
 
-Lemma formula_implies_filter_outputs :
+Lemma sigma_outputs_satisfy_entailed :
   forall db q premise conclusion,
-    formula_implies_on_output db q premise conclusion ->
-    formula_true_on_output db (Sigma premise q) conclusion.
+    query_entails db q premise conclusion ->
+    query_satisfies db (Sigma premise q) conclusion.
 Proof.
 intros db q premise conclusion Himplies t Ht.
 apply Himplies.
@@ -132,14 +132,14 @@ apply Himplies.
       contains_nulls
       contains_nulls_eq
       nil premise t1 t2 Ht12).
-- pose proof (selected_rows_satisfy_filter db q premise t Ht) as Hp.
+- pose proof (sigma_outputs_satisfy_predicate db q premise t Ht) as Hp.
   exact Hp.
 Qed.
 
-Lemma projected_filter_outputs_satisfy_preserved_predicate :
+Lemma pi_sigma_outputs_satisfy_preserved :
   forall db q s f,
-    select_list_preserves_formula db s f ->
-    formula_true_on_output db (Pi s (Sigma f q)) f.
+    select_list_preserves_formula_eval db s f ->
+    query_satisfies db (Pi s (Sigma f q)) f.
 Proof.
 intros db q s f Hpres t Ht.
 unfold eval_query_in_state, eval_query_in_env, Pi in Ht.
@@ -147,19 +147,19 @@ rewrite eval_query_unfold in Ht.
 rewrite Febag.mem_map in Ht.
 destruct Ht as [u [Htu Hu]].
 pose proof (Febag.in_elements_mem _ _ _ Hu) as Hu_mem.
-pose proof (selected_rows_satisfy_filter db q f u Hu_mem) as Hu_f.
+pose proof (sigma_outputs_satisfy_predicate db q f u Hu_mem) as Hu_f.
 unfold eval_formula_in_state.
-rewrite (eval_formula_in_env_eq db nil f t (projected_tuple nil s u) Htu).
+rewrite (eval_formula_in_env_eq_tuple db nil f t (projected_tuple nil s u) Htu).
 change (eval_formula_in_state db (projected_tuple nil s u) f = true).
 rewrite Hpres.
 exact Hu_f.
 Qed.
 
-Lemma projected_filter_outputs_satisfy_implied_predicate :
+Lemma pi_sigma_outputs_satisfy_entailed :
   forall db q s premise conclusion,
-    select_list_preserves_formula db s conclusion ->
-    formula_implies_on_output db q premise conclusion ->
-    formula_true_on_output db (Pi s (Sigma premise q)) conclusion.
+    select_list_preserves_formula_eval db s conclusion ->
+    query_entails db q premise conclusion ->
+    query_satisfies db (Pi s (Sigma premise q)) conclusion.
 Proof.
 intros db q s premise conclusion Hpres Himplies t Ht.
 unfold eval_query_in_state, eval_query_in_env, Pi in Ht.
@@ -167,15 +167,15 @@ rewrite eval_query_unfold in Ht.
 rewrite Febag.mem_map in Ht.
 destruct Ht as [u [Htu Hu]].
 pose proof (Febag.in_elements_mem _ _ _ Hu) as Hu_mem.
-pose proof (formula_implies_filter_outputs db q premise conclusion Himplies u Hu_mem) as Hu_conclusion.
+pose proof (sigma_outputs_satisfy_entailed db q premise conclusion Himplies u Hu_mem) as Hu_conclusion.
 unfold eval_formula_in_state.
-rewrite (eval_formula_in_env_eq db nil conclusion t (projected_tuple nil s u) Htu).
+rewrite (eval_formula_in_env_eq_tuple db nil conclusion t (projected_tuple nil s u) Htu).
 change (eval_formula_in_state db (projected_tuple nil s u) conclusion = true).
 rewrite Hpres.
 exact Hu_conclusion.
 Qed.
 
-Lemma eval_conj_and_true_iff :
+Lemma eval_conj_and :
   forall db env t p h,
     eval_formula_in_env db env t (conj_and p h) =
     (eval_formula_in_env db env t p && eval_formula_in_env db env t h)%bool.
@@ -186,9 +186,85 @@ rewrite eval_sql_formula_unfold.
 apply Bool.is_true_andb.
 Qed.
 
-Lemma redundant_conjunct_under_query_invariant :
+Lemma query_satisfies_conj_l :
   forall db q p h,
-    formula_true_on_output db q h ->
+    query_satisfies db q (conj_and p h) ->
+    query_satisfies db q p.
+Proof.
+intros db q p h Hboth t Ht.
+specialize (Hboth t Ht).
+unfold eval_formula_in_state in *.
+rewrite eval_conj_and in Hboth.
+destruct (eval_formula_in_env db nil t p);
+  destruct (eval_formula_in_env db nil t h);
+  simpl in Hboth; try discriminate; reflexivity.
+Qed.
+
+Lemma query_satisfies_conj_r :
+  forall db q p h,
+    query_satisfies db q (conj_and p h) ->
+    query_satisfies db q h.
+Proof.
+intros db q p h Hboth t Ht.
+specialize (Hboth t Ht).
+unfold eval_formula_in_state in *.
+rewrite eval_conj_and in Hboth.
+destruct (eval_formula_in_env db nil t p);
+  destruct (eval_formula_in_env db nil t h);
+  simpl in Hboth; try discriminate; reflexivity.
+Qed.
+
+Lemma sigma_id_of_query_satisfies :
+  forall db q f,
+    query_satisfies db q f ->
+    query_equiv db (Sigma f q) q.
+Proof.
+intros db q f Htrue.
+unfold query_equiv, eval_query_in_state, Sigma, eval_query_in_env.
+rewrite (@eval_query_unfold TNull relname
+          (@_basesort TNull db)
+          (@_instance TNull db)
+          unknown3
+          contains_nulls
+          nil
+          (@Q_Sigma TNull relname f q)).
+rewrite Febag.nb_occ_equal; intro t.
+rewrite Febag.nb_occ_filter.
+change (@eval_query TNull relname
+          (@_basesort TNull db)
+          (@_instance TNull db)
+          unknown3
+          contains_nulls) with (eval_query_in_env db).
+- match goal with
+  | |- context[(?n * _)%N] => destruct n eqn:Hocc
+  end.
+  + simpl. lia.
+  + assert (Ht : t inBE eval_query_in_state db q).
+    {
+      apply Febag.nb_occ_mem.
+      unfold eval_query_in_state.
+      rewrite Hocc.
+      lia.
+    }
+    change ((N.pos p * (if eval_formula_in_state db t f then 1 else 0))%N =
+            N.pos p).
+    rewrite (Htrue t Ht).
+    lia.
+- intros t1 t2 _ Ht12.
+  unfold eval_formula_in_env, eval_query_in_env.
+  apply (@is_true_eval_f_eq
+    TNull relname
+    (@_basesort TNull db)
+    (@_instance TNull db)
+    unknown3
+    contains_nulls
+    contains_nulls_eq
+    nil f t1 t2 Ht12).
+Qed.
+
+Lemma sigma_drop_redundant_conjunct :
+  forall db q p h,
+    query_satisfies db q h ->
     query_equiv db (Sigma (conj_and p h) q) (Sigma p q).
 Proof.
 intros db q p h Hh.
@@ -207,16 +283,16 @@ apply Febag.filter_eq.
   }
   change (eval_formula_in_env db nil t1 (conj_and p h) =
           eval_formula_in_env db nil t2 p).
-  rewrite eval_conj_and_true_iff.
+  rewrite eval_conj_and.
   replace (eval_formula_in_env db nil t1 h) with (eval_formula_in_state db t1 h)
     by reflexivity.
   rewrite (Hh t1).
   + rewrite Bool.Bool.andb_true_r.
-    apply eval_formula_in_env_eq; assumption.
+    apply eval_formula_in_env_eq_tuple; assumption.
   + exact Ht1mem.
 Qed.
 
-Lemma occurrence_factor_of_andb3 :
+Lemma andb3_indicator_mul_factor :
   forall n outer_value inner_value,
     (n *
       (if match andb3 outer_value inner_value with
@@ -284,7 +360,7 @@ rewrite !Febag.nb_occ_filter.
 - unfold conj_and.
   cbn.
   unfold interp_conj.
-  symmetry; apply occurrence_factor_of_andb3.
+  symmetry; apply andb3_indicator_mul_factor.
 - intros t1 t2 _ Ht12.
   unfold eval_formula_in_env, eval_query_in_env.
   apply (@is_true_eval_f_eq
